More table decomposition lemmas.

src/Examples/DnsServer/AuthoritativeDNSSchema.v
@@ -23,7 +23,7 @@ Definition DnsSchema :=
   Query Structure Schema
         [ relation sRRecords has
                    schema resourceRecordHeading
-          where (fun t t' => t!sNAME = t'!sNAME -> t!sTYPE <> CNAME) ]
+          where (fun t t' => t!sNAME = t'!sNAME -> RDataTypeToRRecordType (t!sRDATA) <> CNAME) ]
         (* constraint on every pair of tuples: if a domain name is an alias, the CNAME record *)
         (* is the only resource record in the table. *)
         enforcing [ ].
