src/Examples/DnsServer/DecomposeSumField.v
@@ -385,14 +385,27 @@ ilist2 (B := @id Type)
     (forall Ridx, Same_set _ (GetUnConstrRelation r_o Ridx)
                            (GetUnConstrRelation (fst r_n) Ridx))
     /\ (forall Ridx tup,
-           IndexedEnsemble_In (GetUnConstrRelation (snd r_n) Ridx) tup
-           ->  IndexedEnsemble_In (GetUnConstrRelation (fst r_n) schemaIdx)
-                                  (Tuple_DecomposeRawQueryStructure_inj' _ _ a a_inj _ tup))
+           In _ (GetUnConstrRelation (snd r_n) Ridx) tup
+           ->  In _ (GetUnConstrRelation (fst r_n) schemaIdx)
+                  {| elementIndex := elementIndex tup;
+                     indexedElement := Tuple_DecomposeRawQueryStructure_inj' _ _ a a_inj _ (indexedElement tup) |})
     /\ (forall tup,
-           IndexedEnsemble_In (GetUnConstrRelation (fst r_n) schemaIdx) tup
-           -> IndexedEnsemble_In (GetUnConstrRelation (snd r_n) (a_proj_index (GetAttributeRaw tup attrIdx))) (Tuple_DecomposeRawQueryStructure_proj' _ _ a _ a_proj tup)).
+           In _ (GetUnConstrRelation (fst r_n) schemaIdx) tup
+           -> In _ (GetUnConstrRelation (snd r_n) (a_proj_index (GetAttributeRaw (indexedElement tup) attrIdx)))
+                 {| elementIndex := elementIndex tup;
+                    indexedElement := Tuple_DecomposeRawQueryStructure_proj' _ _ a _ a_proj (indexedElement tup) |})
+    /\ (forall Ridx Ridx' tup tup' ,
+           In _ (GetUnConstrRelation (snd r_n) Ridx) tup
+           -> In _ (GetUnConstrRelation (snd r_n) Ridx') tup'
+           -> Ridx <> Ridx'
+           -> elementIndex tup <> elementIndex tup')
+    /\ (forall Ridx tup,
+           In IndexedElement (GetUnConstrRelation (snd r_n) Ridx) tup
+           -> a_proj_index (GetAttributeRaw
+                              (Tuple_DecomposeRawQueryStructure_inj' _ _ a a_inj _ (indexedElement tup)) attrIdx) = Ridx)
+    /\ (forall Ridx, FiniteEnsemble (GetUnConstrRelation (snd r_n) Ridx)).
 
-    Definition DecomposeRawQueryStructureSchema_AbsR'
+  Definition DecomposeRawQueryStructureSchema_AbsR'
              {m : nat}
              {qs_schema : QueryStructureSchema}
              ( schemaIdx' : BoundedIndex (QSschemaNames qs_schema))
@@ -446,7 +459,24 @@ Proof.
     rewrite EmptyRefinements.ith_Bounded_BuildEmptyRelations in H.
     simpl in H; unfold IndexedEnsemble_In in H; destruct_ex;
       inversion H.
-Qed.
+    - unfold UnConstrFreshIdx in *; intros.
+      unfold GetUnConstrRelation, DropQSConstraints, QSEmptySpec in H0.
+      rewrite <- ith_imap2 in H0.
+      simpl in H0.
+      rewrite EmptyRefinements.ith_Bounded_BuildEmptyRelations in H0.
+      destruct H0.
+    - unfold UnConstrFreshIdx in *; intros.
+      unfold GetUnConstrRelation, DropQSConstraints, QSEmptySpec in H.
+      rewrite <- ith_imap2 in H.
+      simpl in H.
+      rewrite EmptyRefinements.ith_Bounded_BuildEmptyRelations in H.
+      destruct H.
+    - unfold FiniteEnsemble; eexists nil.
+      unfold GetUnConstrRelation, DropQSConstraints, QSEmptySpec.
+      rewrite <- ith_imap2.
+      rewrite EmptyRefinements.ith_Bounded_BuildEmptyRelations.
+      apply  UnIndexedEnsembleListEquivalence_Empty_set.
+  Qed.
 
 Definition DecomposeRawQueryStructureSchema_Insert_AbsR_neq
              {m : nat}
@@ -494,11 +524,17 @@ Proof.
   - unfold GetUnConstrRelation, UpdateUnConstrRelation in *.
     rewrite !ith_replace2_Index_neq in H1; eauto.
     eapply (proj2 H); eauto.
-Qed.
+  - unfold GetUnConstrRelation, UpdateUnConstrRelation in *.
+    eapply H; eauto.
+  - unfold GetUnConstrRelation, UpdateUnConstrRelation in *.
+    eapply H; eauto.
+  - unfold GetUnConstrRelation, UpdateUnConstrRelation in *.
+    eapply H; eauto.
+  Qed.
 
 Lemma Tuple_DecomposeRawQueryStructure_inj_inverse
       {m : nat}
-      {qs_schema : QueryStructureSchema}
+      {qs_schema : RawQueryStructureSchema}
   : forall (schemaIdx : Fin.t _)
            (attrIdx : Fin.t _)
            (a : Vector.t Type m)
@@ -511,6 +547,15 @@ Lemma Tuple_DecomposeRawQueryStructure_inj_inverse
                                           (Tuple_DecomposeRawQueryStructure_proj' schemaIdx attrIdx a a_proj_index a_proj
                                                                                  tup) = tup.
 Admitted.
+
+  Lemma ith_replace2_Index_eq':
+    forall (A : Type) (B : A -> Type) (m : nat) (n n' : Fin.t m) (As : t A m) (il : ilist2 As) (new_b : B As[@n'])
+           (H : n' = n),
+      ith2 (replace_Index2 As il n' new_b) n = @eq_rect _ _ (fun n => B As[@n]) new_b _ H.
+  Proof.
+    intros.
+    subst; unfold eq_rect; apply ith_replace2_Index_eq.
+  Qed.
 
 Definition DecomposeRawQueryStructureSchema_Insert_AbsR_eq
              {m : nat}
@@ -527,7 +572,8 @@ Definition DecomposeRawQueryStructureSchema_Insert_AbsR_eq
       schemaIdx attrIdx a a_proj_index a_proj a_inj
       r_o r_n
     ->
-    forall tup,
+    forall tup
+      (freshIdx : UnConstrFreshIdx (GetUnConstrRelation (fst r_n) schemaIdx) (elementIndex tup)),
       DecomposeRawQueryStructureSchema_AbsR
         schemaIdx attrIdx a a_proj_index a_proj a_inj
         (UpdateUnConstrRelation r_o schemaIdx (EnsembleInsert tup (GetUnConstrRelation r_o schemaIdx)))
@@ -565,37 +611,176 @@ Definition DecomposeRawQueryStructureSchema_Insert_AbsR_eq
                   Ridx
                   (a_proj_index (GetAttributeRaw (indexedElement tup) attrIdx))); subst.
       rewrite !ith_replace2_Index_eq in H0.
-      destruct H0 as [? [? | ?] ].
-      * destruct tup; injections; econstructor; econstructor.
-        f_equal; simpl.
-        apply Tuple_DecomposeRawQueryStructure_inj_inverse.
-      * destruct (proj1 (proj2 H) (a_proj_index (GetAttributeRaw (indexedElement tup) attrIdx)) tup0).
-        econstructor; eauto.
-        econstructor; econstructor 2; eauto.
+      destruct H0 as [? | ?]; subst.
+      * destruct tup; subst; injections; simpl.
+        econstructor; f_equal; simpl.
+        erewrite <- Tuple_DecomposeRawQueryStructure_inj_inverse.
+        reflexivity.
+      * pose proof (proj1 (proj2 H) (a_proj_index (GetAttributeRaw (indexedElement tup) attrIdx)) tup0).
+        apply H1 in H0.
+        econstructor 2; eauto.
       * rewrite !ith_replace2_Index_neq in H0 by eauto.
-        destruct (proj1 (proj2 H) Ridx tup0 H0); eauto.
-        econstructor; econstructor 2; eauto.
+        pose proof (proj1 (proj2 H) Ridx tup0 H0); eauto.
+        econstructor 2; eauto.
   - unfold GetUnConstrRelation, UpdateUnConstrRelation in *.
     + rewrite !ith_replace2_Index_eq in H0.
-      destruct H0 as [? [? | ?] ]; subst.
+      destruct H0 as [? | ?]; subst.
       * try rewrite !ith_replace2_Index_eq.
         econstructor; econstructor; f_equal.
-      * destruct (proj2 (proj2 H) tup0).
-        econstructor; eauto.
+      * apply (proj1 (proj2 (proj2 H)) tup0) in H0.
         simpl in *.
-        econstructor; simpl.
-        destruct tup; simpl in *.
-        clear r_o H H0 a_inj.
-        unfold In.
-        destruct (fin_eq_dec (a_proj_index (GetAttributeRaw tup0 attrIdx))
-                             (a_proj_index (GetAttributeRaw indexedElement attrIdx))
+        destruct tup0; destruct tup; simpl in *.
+        clear r_o H.
+        destruct (fin_eq_dec (a_proj_index (GetAttributeRaw indexedElement attrIdx))
+                             (a_proj_index (GetAttributeRaw indexedElement0 attrIdx))
                  ); subst;
           [ | rewrite !ith_replace2_Index_neq; eauto].
+        symmetry in e;
+          erewrite ith_replace2_Index_eq' with (H := e).
+        revert H0; clear.
         match goal with
-          |- ith2 (replace_Index2 _ _ ?idx _) ?idx' _ =>
-          assert (idx = idx')
+            |- context[In _ _ ?G] => generalize G; clear
+          end.
+        revert e.
+        match goal with
+          |- context[EnsembleInsert ?t _] =>
+          generalize t
         end.
-Admitted.
+        clear.
+        destruct e; simpl; intros.
+        unfold EnsembleInsert; intuition.
+    - unfold GetUnConstrRelation, UpdateUnConstrRelation in *.
+      destruct (fin_eq_dec
+                  Ridx
+                  (a_proj_index (GetAttributeRaw (indexedElement tup) attrIdx)));
+        destruct (fin_eq_dec
+                    Ridx'
+                    (a_proj_index (GetAttributeRaw (indexedElement tup) attrIdx))); subst.
+      + congruence.
+      + rewrite ith_replace2_Index_eq in H0.
+        rewrite ith_replace2_Index_neq in H1 by eauto.
+        destruct H0 as [? | ?]; subst; simpl.
+        * apply (proj1 (proj2 H)) in H1; apply freshIdx in H1; simpl in *; try omega.
+        * apply H; eauto.
+      + rewrite ith_replace2_Index_neq in H0 by eauto.
+        rewrite ith_replace2_Index_eq in H1.
+        destruct H1 as [? | ?]; subst; simpl.
+        * apply (proj1 (proj2 H)) in H0; apply freshIdx in H0; simpl in *; omega.
+        * apply H; eauto.
+      + rewrite ith_replace2_Index_neq in H0 by eauto.
+        rewrite ith_replace2_Index_neq in H1 by eauto.
+        apply H; eauto.
+    - unfold GetUnConstrRelation, UpdateUnConstrRelation in *.
+      destruct (fin_eq_dec
+                  Ridx
+                  (a_proj_index (GetAttributeRaw (indexedElement tup) attrIdx))).
+      + subst.
+        rewrite ith_replace2_Index_eq in H0.
+        destruct H0 as [? | ?]; subst; simpl.
+        * repeat f_equal.
+          erewrite <- Tuple_DecomposeRawQueryStructure_inj_inverse;
+            reflexivity.
+        * apply H; eauto.
+      + rewrite ith_replace2_Index_neq in H0 by eauto.
+        apply H; eauto.
+    - unfold GetUnConstrRelation, UpdateUnConstrRelation in *.
+      destruct (fin_eq_dec
+                  Ridx
+                  (a_proj_index (GetAttributeRaw (indexedElement tup) attrIdx))).
+      + subst; rewrite ith_replace2_Index_eq.
+        apply FiniteEnsemble_Insert; eauto.
+        * unfold UnConstrFreshIdx in *; simpl in *; intros.
+          eapply (proj1 (proj2 H)) in H0; simpl in H0.
+          apply freshIdx in H0.
+          simpl in H0; eauto.
+        * apply H.
+      + rewrite ith_replace2_Index_neq by eauto.
+        apply H.
+  Qed.
+
+Corollary DecomposeRawQueryStructureSchema_UpdateUnConstrRelationInsertC_eq
+             {m : nat}
+             {qs_schema : QueryStructureSchema}
+             {ResultT}
+  : forall (schemaIdx : Fin.t _)
+           (attrIdx : Fin.t _)
+           (a : Vector.t Type m)
+           (a_proj_index : Vector.nth (AttrList (GetNRelSchemaHeading (qschemaSchemas qs_schema) schemaIdx)) attrIdx -> Fin.t m)
+           (a_proj : forall (attr : Vector.nth _ attrIdx), a[@a_proj_index attr])
+           (a_inj : forall idx, Vector.nth a idx -> Vector.nth (AttrList (GetNRelSchemaHeading (qschemaSchemas qs_schema) schemaIdx)) attrIdx)
+           r_o
+           r_n
+           (k : UnConstrQueryStructure qs_schema -> Comp ResultT)
+           (k' : _ -> Comp ResultT),
+    DecomposeRawQueryStructureSchema_AbsR
+      schemaIdx attrIdx a a_proj_index a_proj a_inj
+      r_o r_n
+    -> forall freshIdx tup,
+        UnConstrFreshIdx (GetUnConstrRelation (fst r_n) schemaIdx) freshIdx
+        -> (forall r_o' r_n',
+               DecomposeRawQueryStructureSchema_AbsR
+                 schemaIdx attrIdx a a_proj_index a_proj a_inj
+                 r_o' r_n'
+               -> refine (k r_o') (k' r_n'))
+        ->
+        refine (r_o' <- UpdateUnConstrRelationInsertC r_o schemaIdx {| elementIndex := freshIdx; indexedElement := tup |};
+                  k r_o')
+               (r_n' <- UpdateUnConstrRelationInsertC (fst r_n) schemaIdx {| elementIndex := freshIdx; indexedElement := tup |};
+                  r_n'' <- UpdateUnConstrRelationInsertC (snd r_n)
+                        (a_proj_index (GetAttributeRaw tup attrIdx))
+                        {| elementIndex := freshIdx;
+                           indexedElement :=
+                             Tuple_DecomposeRawQueryStructure_proj'
+                               _ _ _ _ a_proj
+                               tup |};
+                  k' (r_n', r_n'')).
+  Proof.
+    Local Transparent UpdateUnConstrRelationInsertC.
+    unfold UpdateUnConstrRelationInsertC; intros.
+    repeat rewrite refineEquiv_bind_unit.
+    rewrite H1.
+    reflexivity.
+    simpl.
+    eapply (DecomposeRawQueryStructureSchema_Insert_AbsR_eq H); eauto.
+  Qed.
+
+  Corollary DecomposeRawQueryStructureSchema_UpdateUnConstrRelationInsertC_neq
+            {m : nat}
+            {qs_schema : QueryStructureSchema}
+            {ResultT}
+    : forall (schemaIdx : Fin.t _)
+             (attrIdx : Fin.t _)
+             (a : Vector.t Type m)
+             (a_proj_index : Vector.nth (AttrList (GetNRelSchemaHeading (qschemaSchemas qs_schema) schemaIdx)) attrIdx -> Fin.t m)
+             (a_proj : forall (attr : Vector.nth _ attrIdx), a[@a_proj_index attr])
+             (a_inj : forall idx, Vector.nth a idx -> Vector.nth (AttrList (GetNRelSchemaHeading (qschemaSchemas qs_schema) schemaIdx)) attrIdx)
+             r_o
+             r_n
+             (k : UnConstrQueryStructure qs_schema -> Comp ResultT)
+             (k' : _ -> Comp ResultT),
+      DecomposeRawQueryStructureSchema_AbsR
+        schemaIdx attrIdx a a_proj_index a_proj a_inj
+        r_o r_n
+      -> forall Ridx freshIdx tup,
+        Ridx <> schemaIdx
+        -> UnConstrFreshIdx (GetUnConstrRelation (fst r_n) Ridx) freshIdx
+        -> (forall r_o' r_n',
+               DecomposeRawQueryStructureSchema_AbsR
+                 schemaIdx attrIdx a a_proj_index a_proj a_inj
+                 r_o' r_n'
+               -> refine (k r_o') (k' r_n'))
+        ->
+        refine (r_o' <- UpdateUnConstrRelationInsertC r_o Ridx {| elementIndex := freshIdx; indexedElement := tup |};
+                  k r_o')
+               (r_n' <- UpdateUnConstrRelationInsertC (fst r_n) Ridx {| elementIndex := freshIdx; indexedElement := tup |};
+                  k' (r_n', snd r_n)).
+  Proof.
+    unfold UpdateUnConstrRelationInsertC; intros.
+    repeat rewrite refineEquiv_bind_unit.
+    rewrite H2.
+    reflexivity.
+    simpl; eapply (DecomposeRawQueryStructureSchema_Insert_AbsR_neq H); eauto.
+  Qed.
 
 Lemma UnConstrFreshIdx_Same_Set_Equiv {ElementType} :
   forall (ensemble ensemble' : @IndexedEnsemble ElementType),
@@ -641,63 +826,615 @@ Proof.
   apply (proj1 H Ridx).
 Qed.
 
-Fixpoint Iterate_Equiv_QueryResultComp
-         m
-         {ResultT}
-         (heading : RawHeading)
-         (headings : Fin.t m -> RawHeading)
-         (Ensembles : forall (idx : Fin.t m),
-             @IndexedEnsemble (@RawTuple (headings idx)))
-         (inj_Tuple : forall (idx : Fin.t m),
-             @RawTuple (headings idx)
-             -> @RawTuple heading)
-         (body : @RawTuple heading -> Comp (list ResultT))
-         {struct m}
-  : Comp (list ResultT) :=
-  match m return
-        forall (headings : Fin.t m -> RawHeading),
-          (forall (idx : Fin.t m),
-              @IndexedEnsemble (@RawTuple (headings idx)))
-          -> (forall (idx : Fin.t m),
-                 @RawTuple (headings idx)
-                 -> @RawTuple heading)
-          -> Comp (list ResultT)
-         with
-         | 0 => fun _ _ _ => (ret List.nil)
-         | S m =>
-           fun headings Ensembles inj_Tuple =>
-             res <- QueryResultComp (Ensembles Fin.F1)
-                 (fun tup => body (inj_Tuple Fin.F1 tup));
-             res' <- Iterate_Equiv_QueryResultComp heading
-                  (fun idx => headings (Fin.FS idx))
-                  (fun idx => Ensembles (Fin.FS idx))
-                  (fun idx tup => (inj_Tuple (Fin.FS idx) tup))
-                  body
-             ;
-             ret (List.app res res')
-          end headings Ensembles inj_Tuple.
+  Local Transparent QueryResultComp.
 
-Lemma refine_Iterate_Equiv_QueryResultComp
-  {m : nat}
-  {qs_schema : RawQueryStructureSchema}
-  {ResultT}
-  (schemaIdx : Fin.t _)
-  (body : @RawTuple _ -> Comp (list ResultT))
-  (attrIdx : Fin.t _)
-  (a : Vector.t Type m)
-  (a_proj_index : Vector.nth (AttrList (GetNRelSchemaHeading (qschemaSchemas qs_schema) schemaIdx)) attrIdx -> Fin.t m)
-  (a_proj : forall (attr : Vector.nth _ attrIdx), a[@a_proj_index attr])
-  (a_inj : forall idx, Vector.nth a idx -> Vector.nth (AttrList (GetNRelSchemaHeading (qschemaSchemas qs_schema) schemaIdx)) attrIdx)
-  (r_o : UnConstrQueryStructure qs_schema)
-  (r_n : UnConstrQueryStructure qs_schema * UnConstrQueryStructure (DecomposeRawQueryStructureSchema qs_schema schemaIdx attrIdx a))
-  : DecomposeRawQueryStructureSchema_AbsR schemaIdx attrIdx a a_proj_index a_proj a_inj r_o r_n
-    ->
-    refine (UnConstrQuery_In r_o schemaIdx body)
-           (Iterate_Equiv_QueryResultComp
-              _ _
-              (GetUnConstrRelation (snd r_n))
-              (Tuple_DecomposeRawQueryStructure_inj' _ _ a a_inj) body).
-Admitted.
+  Lemma flatten_CompList_ret:
+    forall (A B : Type) (f : A -> B) (l : list A),
+      refine (ret (map f l))
+             (FlattenCompList.flatten_CompList (map (fun a => ret [(f a)]) l))%list.
+  Proof.
+    induction l; simpl.
+    - reflexivity.
+    - setoid_rewrite <- IHl.
+      repeat setoid_rewrite refineEquiv_bind_unit.
+      simpl; reflexivity.
+  Qed.
+
+    Fixpoint Iterate_Equiv_QueryResultComp
+           m
+           (heading : RawHeading)
+           (headings : Fin.t m -> RawHeading)
+           (Ensembles : forall (idx : Fin.t m),
+               @IndexedEnsemble (@RawTuple (headings idx)))
+           (inj_Tuple : forall (idx : Fin.t m),
+               @RawTuple (headings idx)
+               -> @RawTuple heading)
+           {struct m}
+    : Comp (list (@RawTuple heading)) :=
+    match m return
+          forall (headings : Fin.t m -> RawHeading),
+            (forall (idx : Fin.t m),
+                @IndexedEnsemble (@RawTuple (headings idx)))
+            -> (forall (idx : Fin.t m),
+                   @RawTuple (headings idx)
+                   -> @RawTuple heading)
+            -> Comp (list _)
+    with
+    | 0 => fun _ _ _ => (ret List.nil)
+    | S m =>
+      fun headings Ensembles inj_Tuple =>
+        res <- QueryResultComp (Ensembles Fin.F1)
+            (fun tup => ret [inj_Tuple Fin.F1 tup])%list;
+          res' <- Iterate_Equiv_QueryResultComp heading
+               (fun idx => headings (Fin.FS idx))
+               (fun idx => Ensembles (Fin.FS idx))
+               (fun idx tup => (inj_Tuple (Fin.FS idx) tup))
+          ;
+          ret (List.app res res')
+    end headings Ensembles inj_Tuple.
+
+  Lemma refine_UnIndexedEnsembleListEquivalence_Iterate_Equiv_QueryResultComp
+        m
+        (heading : RawHeading)
+        (headings : Fin.t m -> RawHeading)
+        (Ensembles : forall (idx : Fin.t m),
+            @IndexedEnsemble (@RawTuple (headings idx)))
+        (inj_Tuple : forall (idx : Fin.t m),
+            @RawTuple (headings idx)
+            -> @RawTuple heading)
+
+        (distinctIndexes : forall idx idx' tup tup',
+            idx <> idx'
+            -> Ensembles idx tup
+            -> Ensembles idx' tup'
+            -> elementIndex tup <> elementIndex tup')
+    : refine
+        {queriedList : list RawTuple |
+         UnIndexedEnsembleListEquivalence
+           (fun tup => exists idx tup',
+                tup = {| elementIndex := elementIndex tup';
+                         indexedElement := inj_Tuple idx (indexedElement tup') |}
+                /\ In _ (Ensembles idx) tup')
+           queriedList}
+        (Iterate_Equiv_QueryResultComp heading headings Ensembles inj_Tuple).
+  Proof.
+    revert heading headings Ensembles inj_Tuple distinctIndexes.
+    induction m; simpl; intros; intros ? ?.
+    - computes_to_inv; subst; computes_to_econstructor.
+      unfold UnIndexedEnsembleListEquivalence; eexists nil; simpl;
+        intuition eauto.
+      unfold In in H; destruct_ex; intuition subst.
+      inversion x0.
+      constructor.
+    - unfold QueryResultComp in H.
+      computes_to_inv; subst.
+      eapply IHm in H'; computes_to_inv; clear IHm.
+      apply flatten_CompList_ret in H'0; computes_to_inv; subst.
+      computes_to_econstructor. unfold UnIndexedEnsembleListEquivalence in *;
+                                  destruct_ex; intuition; subst.
+      rewrite map_map.
+      replace (fun x1 : IndexedElement => inj_Tuple Fin.F1 (indexedElement x1))
+      with (fun x1 : IndexedElement => indexedElement {| elementIndex := elementIndex x1;
+                                                         indexedElement := inj_Tuple Fin.F1 (indexedElement x1) |}) by
+          (apply functional_extensionality; reflexivity).
+      rewrite <- map_map.
+      eexists (_ ++ _)%list.
+      rewrite map_app; intuition eauto.
+      + unfold In in *; destruct_ex; intuition subst.
+        revert headings Ensembles inj_Tuple distinctIndexes x0 x H0 H4 H2 H5 x3 H3.
+        pattern m, x2.
+        eapply Fin.caseS; clear m x2; intros.
+        * simpl in *; apply H0 in H3; apply in_or_app; left.
+          eapply in_map with
+          (f := (fun x1 : IndexedElement =>
+                   {| elementIndex := elementIndex x1;
+                      indexedElement := inj_Tuple Fin.F1 (indexedElement x1) |})) in H3.
+          apply H3.
+        * apply in_or_app; right.
+          eapply H2; eexists _,_; intuition eauto.
+      + apply in_app_or in H; unfold In in *; destruct_ex; intuition subst.
+        * apply in_map_iff in H1; destruct_ex; intuition subst.
+          eexists _, _; intuition eauto.
+          eapply H0; eauto.
+        * eapply H2 in H1.
+          destruct_ex; intuition subst.
+          eexists _, _; intuition eauto.
+      + rewrite map_app.
+        eapply NoDup_app_in_iff; intuition.
+        revert H4; clear; induction x0; simpl; intros; econstructor;
+          inversion H4; subst; eauto.
+        intro; apply H1; revert H; clear; induction x0; simpl; intuition auto.
+        rewrite map_map in H1.
+        apply in_map_iff in H; apply in_map_iff in H1.
+        destruct_ex; intuition; subst.
+        eapply H2 in H6; eapply H0 in H7.
+        destruct H6 as [? [? [? ?] ] ]; simpl in *; subst;
+          simpl in *.
+        eapply (distinctIndexes Fin.F1 (Fin.FS x1)); eauto.
+        intros; discriminate.
+      + intros; eapply distinctIndexes; eauto.
+        intro; apply H0.
+        apply Fin.FS_inj; eauto.
+  Qed.
+
+  Fixpoint Iterate_Equiv_QueryResultComp_body
+           m
+           {ResultT}
+           (heading : RawHeading)
+           (headings : Fin.t m -> RawHeading)
+           (Ensembles : forall (idx : Fin.t m),
+               @IndexedEnsemble (@RawTuple (headings idx)))
+           (inj_Tuple : forall (idx : Fin.t m),
+               @RawTuple (headings idx)
+               -> @RawTuple heading)
+           (body : @RawTuple heading -> Comp (list ResultT))
+           {struct m}
+    : Comp (list ResultT) :=
+    match m return
+          forall (headings : Fin.t m -> RawHeading),
+            (forall (idx : Fin.t m),
+                @IndexedEnsemble (@RawTuple (headings idx)))
+            -> (forall (idx : Fin.t m),
+                   @RawTuple (headings idx)
+                   -> @RawTuple heading)
+            -> Comp (list ResultT)
+    with
+    | 0 => fun _ _ _ => (ret List.nil)
+    | S m =>
+      fun headings Ensembles inj_Tuple =>
+        res <- QueryResultComp (Ensembles Fin.F1)
+            (fun tup => body (inj_Tuple Fin.F1 tup));
+          res' <- Iterate_Equiv_QueryResultComp_body heading
+               (fun idx => headings (Fin.FS idx))
+               (fun idx => Ensembles (Fin.FS idx))
+               (fun idx tup => (inj_Tuple (Fin.FS idx) tup))
+               body
+          ;
+          ret (List.app res res')
+    end headings Ensembles inj_Tuple.
+
+  Lemma refine_Iterate_Equiv_QueryResultComp_body
+        m
+        {ResultT : Type}
+        (heading : RawHeading)
+        (headings : Fin.t m -> RawHeading)
+        (Ensembles : forall (idx : Fin.t m),
+            @IndexedEnsemble (@RawTuple (headings idx)))
+        (inj_Tuple : forall (idx : Fin.t m),
+            @RawTuple (headings idx)
+            -> @RawTuple heading)
+        (body : @RawTuple heading -> Comp (list ResultT))
+    : refineEquiv
+        (results <- Iterate_Equiv_QueryResultComp heading headings Ensembles inj_Tuple;
+           FlattenCompList.flatten_CompList (map body results))
+        (Iterate_Equiv_QueryResultComp_body heading headings Ensembles inj_Tuple body).
+  Proof.
+    split.
+    - induction m; simpl.
+      + simplify with monad laws.
+        simpl; reflexivity.
+      + simplify with monad laws.
+        setoid_rewrite <- IHm.
+        repeat setoid_rewrite refineEquiv_bind_bind.
+        f_equiv; intro.
+        rewrite refineEquiv_swap_bind.
+        rewrite (refineEquiv_swap_bind
+                   (FlattenCompList.flatten_CompList (map (fun tup : RawTuple => body (inj_Tuple Fin.F1 tup)) a))).
+        f_equiv; intro.
+        induction a; simpl; simplify with monad laws.
+        * setoid_rewrite refineEquiv_bind_unit.
+          simpl; setoid_rewrite refineEquiv_unit_bind.
+          reflexivity.
+        * repeat setoid_rewrite refineEquiv_bind_bind.
+          simpl.
+          rewrite refineEquiv_swap_bind.
+          f_equiv; intro.
+          rewrite <- refineEquiv_bind_bind, IHa.
+          simplify with monad laws.
+          setoid_rewrite refineEquiv_bind_unit.
+          setoid_rewrite <- List.app_assoc.
+          reflexivity.
+    - induction m; simpl.
+      + setoid_rewrite refineEquiv_bind_unit.
+        simpl; reflexivity.
+      + repeat setoid_rewrite refineEquiv_bind_bind.
+        setoid_rewrite IHm.
+        repeat setoid_rewrite refineEquiv_bind_bind.
+        f_equiv; intro.
+        rewrite refineEquiv_swap_bind.
+        setoid_rewrite (refineEquiv_swap_bind
+                          _
+                          (Iterate_Equiv_QueryResultComp heading (fun idx : Fin.t m => headings (Fin.FS idx))
+                                                         (fun idx : Fin.t m => Ensembles (Fin.FS idx))
+                                                         (fun (idx : Fin.t m) (tup : RawTuple) => inj_Tuple (Fin.FS idx) tup))).
+        setoid_rewrite refineEquiv_bind_unit.
+        f_equiv; intro.
+        revert a0.
+        induction a; simpl; intros; simplify with monad laws.
+        * setoid_rewrite refineEquiv_bind_unit.
+          reflexivity.
+        * repeat setoid_rewrite refineEquiv_bind_bind.
+          repeat setoid_rewrite refineEquiv_bind_unit.
+          setoid_rewrite map_app.
+          simpl.
+          rewrite <- (refineEquiv_swap_bind (body (inj_Tuple Fin.F1 a))).
+          f_equiv; intro.
+          setoid_rewrite map_app in IHa.
+          setoid_rewrite <- refineEquiv_bind_bind; rewrite <- IHa.
+          repeat setoid_rewrite refineEquiv_bind_bind.
+          setoid_rewrite refineEquiv_bind_unit.
+          setoid_rewrite <- List.app_assoc.
+          f_equiv; intro.
+  Qed.
+
+  Lemma refine_UnIndexedEnsembleListEquivalence {A}
+    : forall s s',
+      (forall l, UnIndexedEnsembleListEquivalence s' l
+                 -> UnIndexedEnsembleListEquivalence s l)
+      -> refine {queriedList : list A | UnIndexedEnsembleListEquivalence s queriedList}
+                {queriedList : list A | UnIndexedEnsembleListEquivalence s' queriedList}.
+  Proof.
+    intros ? ?; computes_to_inv; computes_to_econstructor.
+    computes_to_inv.
+    eauto.
+  Qed.
+
+  Lemma UnIndexedEnsembleListEquivalence_app {A} :
+    forall (P Q : IndexedEnsemble) (l l' : list A),
+      Disjoint _ (fun idx => exists tup,
+                      In _ P {| elementIndex := idx;
+                                indexedElement := tup |})
+               (fun idx => exists tup,
+                    In _ Q {| elementIndex := idx;
+                              indexedElement := tup |})
+      -> UnIndexedEnsembleListEquivalence P l
+      -> UnIndexedEnsembleListEquivalence Q l'
+      -> UnIndexedEnsembleListEquivalence (Union _ P Q) (l ++ l').
+  Proof.
+    unfold UnIndexedEnsembleListEquivalence; intros.
+    destruct_ex; intuition.
+    eexists (x0 ++ x)%list; intuition; eauto.
+    - rewrite map_app; congruence.
+    - apply in_or_app.
+      setoid_rewrite <- H1; setoid_rewrite <- H3;
+        destruct H4; intuition.
+    - apply in_app_or in H4.
+      setoid_rewrite <- H1 in H4; setoid_rewrite <- H3 in H4.
+      intuition.
+    - rewrite map_app; apply NoDup_app_in_iff; intuition.
+      apply in_map_iff in H4; apply in_map_iff in H7;
+        destruct_ex; intuition; subst.
+      apply H1 in H10; apply H3 in H9.
+      inversion H; subst.
+      eapply (H0 (elementIndex x2)).
+      destruct x3; destruct x2; subst; simpl in *.
+      econstructor; unfold In.
+      eexists; eauto.
+      rewrite H4; eexists; eauto.
+  Qed.
+
+  Lemma refine_UnConstrQuery_In_DecomposeRawQueryStructureSchema_AbsR
+        {m : nat}
+        {qs_schema : RawQueryStructureSchema}
+        {ResultT}
+        (schemaIdx : Fin.t _)
+        (body : @RawTuple _ -> Comp (list ResultT))
+        (attrIdx : Fin.t _)
+        (a : Vector.t Type m)
+        (a_proj_index : Vector.nth (AttrList (GetNRelSchemaHeading (qschemaSchemas qs_schema) schemaIdx)) attrIdx -> Fin.t m)
+        (a_proj : forall (attr : Vector.nth _ attrIdx), a[@a_proj_index attr])
+        (a_inj : forall idx, Vector.nth a idx -> Vector.nth (AttrList (GetNRelSchemaHeading (qschemaSchemas qs_schema) schemaIdx)) attrIdx)
+        (r_o : UnConstrQueryStructure qs_schema)
+        (r_n : UnConstrQueryStructure qs_schema * UnConstrQueryStructure (DecomposeRawQueryStructureSchema qs_schema schemaIdx attrIdx a))
+    : DecomposeRawQueryStructureSchema_AbsR schemaIdx attrIdx a a_proj_index a_proj a_inj r_o r_n
+      ->
+      refine (UnConstrQuery_In r_o schemaIdx body) (UnConstrQuery_In (fst r_n) schemaIdx body).
+  Proof.
+    intros.
+    unfold UnConstrQuery_In, QueryResultComp; f_equiv.
+    rewrite refine_UnIndexedEnsembleListEquivalence.
+    reflexivity.
+    intros.
+    eapply UnIndexedEnsembleListEquivalence_Same_set; eauto.
+    destruct H.
+    unfold Same_set in *; intuition eauto.
+    apply H.
+    apply H.
+  Qed.
+
+  Lemma refine_Iterate_Equiv_QueryResultComp
+        {m : nat}
+        {qs_schema : RawQueryStructureSchema}
+        {ResultT}
+        (schemaIdx : Fin.t _)
+        (body : @RawTuple _ -> Comp (list ResultT))
+        (attrIdx : Fin.t _)
+        (a : Vector.t Type m)
+        (a_proj_index : Vector.nth (AttrList (GetNRelSchemaHeading (qschemaSchemas qs_schema) schemaIdx)) attrIdx -> Fin.t m)
+        (a_proj : forall (attr : Vector.nth _ attrIdx), a[@a_proj_index attr])
+        (a_inj : forall idx, Vector.nth a idx -> Vector.nth (AttrList (GetNRelSchemaHeading (qschemaSchemas qs_schema) schemaIdx)) attrIdx)
+        (r_o : UnConstrQueryStructure qs_schema)
+        (r_n : UnConstrQueryStructure qs_schema * UnConstrQueryStructure (DecomposeRawQueryStructureSchema qs_schema schemaIdx attrIdx a))
+    : DecomposeRawQueryStructureSchema_AbsR schemaIdx attrIdx a a_proj_index a_proj a_inj r_o r_n
+      ->
+      refine (UnConstrQuery_In r_o schemaIdx body)
+             (Iterate_Equiv_QueryResultComp_body
+                _ _
+                (GetUnConstrRelation (snd r_n))
+                (Tuple_DecomposeRawQueryStructure_inj' _ _ a a_inj) body).
+  Proof.
+    intros.
+    erewrite refine_UnConstrQuery_In_DecomposeRawQueryStructureSchema_AbsR by eassumption.
+    rewrite <- refine_Iterate_Equiv_QueryResultComp_body.
+    unfold UnConstrQuery_In, QueryResultComp; f_equiv.
+    rewrite refine_UnIndexedEnsembleListEquivalence.
+    - unfold DecomposeRawQueryStructureSchema; simpl.
+      intros; rewrite <- refine_UnIndexedEnsembleListEquivalence_Iterate_Equiv_QueryResultComp.
+      + reflexivity.
+      + intros; destruct H as [? [? [? [? ?] ] ] ].
+        intro; pose proof (H5 _ _ _ _ H1 H2 H0); simpl in *; eauto.
+    - unfold UnIndexedEnsembleListEquivalence; simpl; intros.
+      destruct_ex; intuition; subst.
+      eexists x; intuition eauto.
+      apply H in H1.
+      apply H0.
+      eexists _, _; split; eauto.
+      simpl; destruct x0; simpl; f_equal.
+      symmetry; eapply Tuple_DecomposeRawQueryStructure_inj_inverse.
+      unfold In in *; apply H0 in H1; destruct_ex; intuition; subst.
+      apply (proj1 (proj2 H)) in H4; eassumption.
+  Qed.
+
+    Lemma refine_Query_Where_Cond :
+    forall (ResultT : Type) (P Q : Prop)
+           (body : Comp (list ResultT)),
+      (P <-> Q)
+      -> refine (Query_Where P body)
+                (Query_Where Q body).
+  Proof.
+    unfold pointwise_relation, Query_Where; intros.
+    intros ? ?; intuition; computes_to_inv; computes_to_econstructor.
+    intuition; intros.
+  Qed.
+
+  Lemma refine_flatten_CompList_func' :
+    forall (A B : Type) (l : list A) (f f' : A -> Comp (list B)),
+      (forall v, List.In v l -> refine (f v) (f' v))
+      -> refine (FlattenCompList.flatten_CompList (map f l)) (FlattenCompList.flatten_CompList (map f' l)).
+  Proof.
+    induction l; simpl; intros.
+    - reflexivity.
+    - rewrite H by eauto.
+      f_equiv; intro.
+      rewrite IHl by eauto.
+      reflexivity.
+  Qed.
+
+  Lemma refine_Query_Where_True_Cond :
+    forall (ResultT : Type) (P : Prop )
+           (body : Comp (list ResultT)),
+      P
+      -> refine (Query_Where P body) body.
+  Proof.
+    intros.
+    etransitivity; intro.
+    apply refine_Query_Where_Cond with (Q := True).
+    intuition; intros.
+    intros; computes_to_econstructor; intuition.
+  Qed.
+
+  Lemma refine_Query_Where_False_Cond :
+    forall (ResultT : Type) (P : Prop )
+           (body : Comp (list ResultT)),
+      ~ P
+      -> refine (Query_Where P body) (ret nil).
+  Proof.
+    intros.
+    etransitivity; intro.
+    apply refine_Query_Where_Cond with (Q := False).
+    intuition; intros.
+    intros; computes_to_econstructor; intuition;
+      computes_to_inv; eauto.
+  Qed.
+
+  Lemma flatten_CompList_nil':
+  forall (A B : Type)(seq : list A),
+    refine (FlattenCompList.flatten_CompList (map (fun _ => ret nil) seq)) (ret (@nil B)).
+  Proof.
+    induction seq; simpl; unfold refine; intros; computes_to_inv; subst; eauto.
+  Qed.
+
+  Lemma refine_QueryResultComp_body_Where_False
+        {ResultT : Type}
+        {heading}
+        (body : @RawTuple heading -> Comp (list ResultT))
+        P R
+    :
+      (forall tup, In _ R tup -> ~ P (indexedElement tup))
+      -> FiniteEnsemble R
+      -> refine (QueryResultComp R (fun tup => Where (P tup) (body tup)))
+                (ret nil).
+  Proof.
+    intros; unfold QueryResultComp.
+    destruct H0.
+    refine pick val _; eauto.
+    simplify with monad laws.
+    rewrite refine_flatten_CompList_func' with (f' := fun _ => ret nil).
+    apply flatten_CompList_nil'.
+    intros; computes_to_econstructor; computes_to_inv; subst;
+      intuition.
+    unfold UnIndexedEnsembleListEquivalence in H0; destruct_ex;
+        intuition; subst.
+      apply in_map_iff in H1; destruct_ex; intuition; subst.
+      apply H in H2; intuition.
+      apply H0; eauto.
+  Qed.
+
+  Lemma refine_Iterate_Equiv_QueryResultComp_body_Where_False
+        m
+        {ResultT : Type}
+        (heading : RawHeading)
+        (headings : Fin.t m -> RawHeading)
+        (Ensembles : forall (idx : Fin.t m),
+            @IndexedEnsemble (@RawTuple (headings idx)))
+        (inj_Tuple : forall (idx : Fin.t m),
+            @RawTuple (headings idx)
+            -> @RawTuple heading)
+        (FiniteEnsembles : forall idx, FiniteEnsemble (Ensembles idx))
+        (body : @RawTuple heading -> Comp (list ResultT))
+        P
+    :
+      (forall idx tup, In _ (Ensembles idx) tup -> ~ P (inj_Tuple idx (indexedElement tup)))
+      -> refine
+        (Iterate_Equiv_QueryResultComp_body heading headings Ensembles inj_Tuple
+                                            (fun tup : RawTuple => Where (P tup)
+                                                                         (body tup) ))
+                                            (ret nil).
+  Proof.
+    induction m; simpl; intros.
+    - reflexivity.
+    - rewrite refine_QueryResultComp_body_Where_False; eauto.
+      simplify with monad laws.
+      apply IHm; eauto.
+  Qed.
+
+  Lemma refine_Iterate_Equiv_QueryResultComp_body_Where_And_eq
+        m
+        {ResultT : Type}
+        (heading : RawHeading)
+    : forall (headings : Fin.t m -> RawHeading)
+        (Ensembles : forall (idx : Fin.t m),
+            @IndexedEnsemble (@RawTuple (headings idx)))
+        (inj_Tuple : forall (idx : Fin.t m),
+            @RawTuple (headings idx)
+            -> @RawTuple heading)
+        (FiniteEnsembles : forall idx, FiniteEnsemble (Ensembles idx))
+        (body : @RawTuple heading -> Comp (list ResultT))
+        idx
+        P Q,
+      (forall idx',
+          idx <> idx'
+          -> forall tup,
+            In _ (Ensembles idx') tup
+            -> ~ (P (inj_Tuple _ (indexedElement tup))))
+      -> (forall tup,
+             In _ (Ensembles idx) tup
+             -> P (inj_Tuple _ (indexedElement tup)))
+      -> refine
+           (Iterate_Equiv_QueryResultComp_body
+              heading headings Ensembles inj_Tuple
+              (fun tup => Where (P tup /\ Q tup)
+                                (body tup)))
+           (QueryResultComp (Ensembles idx)
+                            (fun tup => Where (Q (inj_Tuple _ tup))
+                                              (body (inj_Tuple idx tup)))).
+  Proof.
+      induction m; simpl; intros.
+      - intros; inversion idx.
+      - destruct (fin_eq_dec idx Fin.F1).
+        + etransitivity.
+          * apply refine_under_bind_both; intros.
+            apply refine_under_bind; intros.
+            eapply refine_flatten_CompList_func'.
+            intros; rewrite (refine_Query_Where_Cond (Q := Q (inj_Tuple _ v))).
+            finish honing.
+            intros; computes_to_inv; unfold UnIndexedEnsembleListEquivalence in H1;
+              destruct_ex; intuition; subst.
+            apply in_map_iff in H2; destruct_ex; intuition; subst.
+            apply H1 in H6; apply H0 in H6; intuition.
+            rewrite e.
+            rewrite refine_Iterate_Equiv_QueryResultComp_body_Where_False.
+            simplify with monad laws;
+              rewrite app_nil_r; finish honing.
+            intuition eauto.
+            unfold not; intros; eapply H; intuition eauto.
+            rewrite e in H4; discriminate.
+          * simplify with monad laws.
+            unfold UnConstrQuery_In, QueryResultComp.
+            rewrite e.
+            reflexivity.
+        + rewrite refine_QueryResultComp_body_Where_False.
+          * simplify with monad laws.
+            revert IHm headings Ensembles inj_Tuple FiniteEnsembles P H H0 n; pattern m, idx.
+            apply Fin.caseS; simpl; intros.
+            congruence.
+            apply (IHm (fun n => headings (Fin.FS n))
+                            (fun n => Ensembles (Fin.FS n))
+                            (fun n tup => inj_Tuple (Fin.FS n) tup));
+              intros; eauto.
+            intro.
+            eapply (H (Fin.FS idx')); eauto.
+            intro; apply H1; apply Fin.FS_inj; eauto.
+          * unfold not; intros.
+            eapply H; intuition eauto.
+          * apply FiniteEnsembles.
+  Qed.
+
+  Lemma refine_QueryIn_Where
+                    {m : nat}
+        {qs_schema : RawQueryStructureSchema}
+        {ResultT}
+        (schemaIdx : Fin.t _)
+        (body : @RawTuple _ -> Comp (list ResultT))
+        (attrIdx : Fin.t _)
+        (a : Vector.t Type m)
+        (a_proj_index : Vector.nth (AttrList (GetNRelSchemaHeading (qschemaSchemas qs_schema) schemaIdx)) attrIdx -> Fin.t m)
+        (a_proj : forall (attr : Vector.nth _ attrIdx), a[@a_proj_index attr])
+        (a_inj : forall idx, Vector.nth a idx -> Vector.nth (AttrList (GetNRelSchemaHeading (qschemaSchemas qs_schema) schemaIdx)) attrIdx)
+        (r_o : UnConstrQueryStructure qs_schema)
+        (r_n : UnConstrQueryStructure qs_schema * UnConstrQueryStructure (DecomposeRawQueryStructureSchema qs_schema schemaIdx attrIdx a))
+        idx
+        Q
+    : DecomposeRawQueryStructureSchema_AbsR schemaIdx attrIdx a a_proj_index a_proj a_inj r_o r_n
+      ->
+      refine (UnConstrQuery_In r_o schemaIdx
+                               (fun tup => Where (a_proj_index (GetAttributeRaw tup attrIdx) =  idx
+                                                  /\ Q tup)
+                                                 (body tup)))
+             (UnConstrQuery_In (snd r_n) idx (fun tup =>
+                                                         Where (Q (Tuple_DecomposeRawQueryStructure_inj' _ _ _ a_inj _ tup))
+                                                               (body
+                                                               (Tuple_DecomposeRawQueryStructure_inj' _ _ _ a_inj _ tup)))).
+  Proof.
+    intros; rewrite (@refine_Iterate_Equiv_QueryResultComp m); eauto.
+    apply refine_Iterate_Equiv_QueryResultComp_body_Where_And_eq  with
+    (idx := idx); eauto.
+    - intros; apply H.
+    - intros; apply H in H1; rewrite H1; congruence.
+    - intros; apply H; eauto.
+  Qed.
+
+  Corollary refine_QueryIn_Where_True
+            {m : nat}
+        {qs_schema : RawQueryStructureSchema}
+        {ResultT}
+        (schemaIdx : Fin.t _)
+        (body : @RawTuple _ -> Comp (list ResultT))
+        (attrIdx : Fin.t _)
+        (a : Vector.t Type m)
+        (a_proj_index : Vector.nth (AttrList (GetNRelSchemaHeading (qschemaSchemas qs_schema) schemaIdx)) attrIdx -> Fin.t m)
+        (a_proj : forall (attr : Vector.nth _ attrIdx), a[@a_proj_index attr])
+        (a_inj : forall idx, Vector.nth a idx -> Vector.nth (AttrList (GetNRelSchemaHeading (qschemaSchemas qs_schema) schemaIdx)) attrIdx)
+        (r_o : UnConstrQueryStructure qs_schema)
+        (r_n : UnConstrQueryStructure qs_schema * UnConstrQueryStructure (DecomposeRawQueryStructureSchema qs_schema schemaIdx attrIdx a))
+        idx
+    : DecomposeRawQueryStructureSchema_AbsR schemaIdx attrIdx a a_proj_index a_proj a_inj r_o r_n
+      -> refine (UnConstrQuery_In r_o schemaIdx
+                               (fun tup => Where (a_proj_index (GetAttributeRaw tup attrIdx) = idx)
+                                                 (body tup)))
+             (UnConstrQuery_In (snd r_n) idx (fun tup =>
+                                                         body
+                                                           (Tuple_DecomposeRawQueryStructure_inj' _ _ _ a_inj _ tup))).
+  Proof.
+    etransitivity.
+    apply refine_UnConstrQuery_In; intro.
+    apply refine_Query_Where_Cond with
+    (Q := (a_proj_index (GetAttributeRaw a0 attrIdx) = idx) /\ True);
+      intuition.
+    setoid_rewrite refine_QueryIn_Where; eauto.
+    apply refine_UnConstrQuery_In; intro.
+    apply refine_Query_Where_True_Cond; eauto.
+  Qed.
 
 Arguments DecomposeRawQueryStructureSchema : simpl never.
 Arguments DecomposeRawQueryStructureSchema_AbsR : simpl never.
@@ -708,7 +1445,7 @@ Arguments SumType_index : simpl never.
 Arguments Vector.nth _ _ _ !_ / .
 
 Definition EnumIDs := ["A"; "NS"; "CNAME"; "SOA" ].
-Definition EnumID := BoundedString EnumIDs.
+Definition EnumID := Fin.t 4.
 Definition EnumTypes := [nat : Type; string : Type; nat : Type; list nat : Type].
 Definition EnumType := SumType EnumTypes.
 
@@ -733,7 +1470,7 @@ Definition EnumType := SumType EnumTypes.
 
             Def Method1 "Process" (this : rep) (p : EnumID) : rep * list _ :=
               results <- For (r in this!"foo")
-                      Where (r!"BID" = p)
+                      Where ( (SumType_index _ r!"B") = p)
                       Return r;
           ret (this, results)}.
 
@@ -749,27 +1486,20 @@ Definition EEImpl : FullySharpened EESpec.
       apply DecomposeRawQueryStructureSchema_empty_AbsR.
     }
     { (* Insert *)
-      unfold DecomposeRawQueryStructureSchema_AbsR' in *.
       simpl in *; simplify with monad laws; cbv beta; simpl.
       rewrite (refine_UnConstrFreshIdx_DecomposeRawQueryStructureSchema_AbsR_Equiv H0 Fin.F1).
       unfold H; eapply refine_under_bind; intros.
       apply refine_under_bind_both; intros.
       apply refine_pick_val.
       eapply (DecomposeRawQueryStructureSchema_Insert_AbsR_eq H0).
+      computes_to_inv; apply H1.
       finish honing.
     }
     { (* Query *)
-      unfold DecomposeRawQueryStructureSchema_AbsR' in *.
       simpl in *; simplify with monad laws; cbv beta; simpl.
       rewrite refine_For; simplify with monad laws.
-      rewrite (refine_Iterate_Equiv_QueryResultComp _ H0).
+      rewrite (refine_QueryIn_Where_True _ H0).
       simpl.
-      simplify with monad laws.
-      unfold Tuple_DecomposeRawQueryStructure_inj'.
-      simpl.
-      unfold GetAttributeRaw; simpl.
-      unfold icons2; simpl.
-      unfold ilist2_tl, ilist2_hd; simpl.
       (* More refinements here. *)
 Abort.
 End DecomposeEnumField.
