src/Computation/ListComputations.v
@@ -142,3 +142,47 @@ Proof.
   setoid_rewrite refine_filtered_list with (P_dec := DecideableEnsembleUpperBound f ns).
   reflexivity.
 Qed.
+
+Lemma refine_ListComprehension_Equiv {A}
+  : forall (As : list A)
+           (P Q : A -> Prop),
+    (forall a, P a <-> Q a)
+    -> refine (⟦element in As | P element ⟧)
+              (⟦element in As | Q element ⟧).
+Proof.
+  induction As; simpl; intros; eauto.
+  - reflexivity.
+  - rewrite IHAs; eauto.
+    apply refine_bind.
+    reflexivity.
+    intros ? ? ?.
+    computes_to_inv; destruct v0; simpl in *.
+    + apply (@BindComputes _ _ _ _ true); eauto.
+      computes_to_econstructor; simpl; eauto.
+      apply H; assumption.
+    + apply (@BindComputes _ _ _ _ false); eauto.
+    computes_to_econstructor;
+      simpl; intros.
+    intro; apply H0.
+    apply H; eassumption.
+Qed.
+
+
+Lemma refine_FindUpperBound {A B}
+  : forall (op : B -> B -> Prop)
+           (op_trans : forall b b' b'', op b b' -> op b' b'' -> op b b'')
+           (bound : B)
+           (As As' : list A)
+           (f : A -> B),
+    (forall a, List.In a As' -> op (f a) bound)
+    -> (exists a, List.In a As' /\ f a = bound)
+    -> refine (⟦element in As | UpperBound (fun a a' => op (f a) (f a')) As' element ⟧)
+              (⟦element in As | op bound (f element) ⟧).
+Proof.
+  intros.
+  unfold UpperBound.
+  apply refine_ListComprehension_Equiv.
+  split; intros.
+  - destruct H0; intuition eauto; subst; eauto.
+  - eapply op_trans; eauto.
+Qed.
