src/Examples/DnsServer/AuthoritativeDNSServer.v
@@ -26,10 +26,11 @@ Require Import
         Fiat.BinEncoders.Env.Lib2.DomainNameOpt.
 
 Require Import Fiat.Examples.DnsServer.Packet
-        Fiat.Examples.DnsServer.DecomposeEnumField
+        Fiat.Examples.DnsServer.DecomposeSumField
         Fiat.Examples.DnsServer.DnsLemmas
         Fiat.Examples.DnsServer.DnsAutomation
         Fiat.Examples.DnsServer.AuthoritativeDNSSchema.
+
 
 Section BinaryDns.
 
@@ -66,7 +67,7 @@ Definition DnsSpec : ADT DnsSig :=
             If (is_empty results) (* Are there any matching records? *)
             Then ret (buildempty true ``"NXDomain" p) (* No matching records, set name error *)
             Else
-            (IfDec (List.Forall (fun r : resourceRecord => n = r!sNAME) results) (* If the record's QNAME is an exact match  *)
+            (IfDec (List.Forall (fun r : resourceRecord => r!sNAME = n) results) (* If the record's QNAME is an exact match  *)
               Then
               b <- SingletonSet (fun b : CNAME_Record =>      (* If the record is a CNAME, *)
                                    List.In (A := resourceRecord) b results
@@ -77,7 +78,7 @@ Definition DnsSpec : ADT DnsSig :=
                   ret (add_answer p' b') (* Add the CNAME RR to the answer section *)
                 Else     (* Copy the records with the correct QTYPE into the answer *)
                          (* section of an empty response *)
-                (results <- ⟦ element in results | QType_match (element!sTYPE) (p!"question"!"qtype") ⟧;
+                (results <- ⟦ element in results | QType_match (RDataTypeToRRecordType element!sRDATA) (p!"question"!"qtype") ⟧;
                   ret (add_answers results (buildempty true ``"NoError" p)))
               Else (* prefix but record's QNAME not an exact match *)
                 (* return all the prefix records that are nameserver records -- *)
@@ -93,404 +94,6 @@ Definition DnsSpec : ADT DnsSig :=
        ret (this, Some (fst b'))
            Else ret (this, None)
            }.
-
-Lemma DropQSConstraints_AbsR_SatisfiesTupleConstraints
-  : forall {qs_schema} r_o r_n,
-    @DropQSConstraints_AbsR qs_schema r_o r_n
-    -> forall idx tup tup',
-      elementIndex tup <> elementIndex tup'
-      -> GetUnConstrRelation r_n idx tup
-      -> GetUnConstrRelation r_n idx tup'
-      -> SatisfiesTupleConstraints idx (indexedElement tup) (indexedElement tup').
-Proof.
-  intros. rewrite <- H in *.
-  unfold SatisfiesTupleConstraints, GetNRelSchema,
-  GetUnConstrRelation, DropQSConstraints in *.
-  generalize (rawTupleconstr (ith2 (rawRels r_o) idx)).
-  rewrite <- ith_imap2 in *.
-  destruct (tupleConstraints (Vector.nth (qschemaSchemas qs_schema) idx)); eauto.
-Qed.
-
-Lemma DropQSConstraints_AbsR_SatisfiesAttribute
-  : forall {qs_schema} r_o r_n,
-    @DropQSConstraints_AbsR qs_schema r_o r_n
-    -> forall idx tup,
-      GetUnConstrRelation r_n idx tup
-      -> SatisfiesAttributeConstraints idx (indexedElement tup).
-Proof.
-  intros. rewrite <- H in *.
-  unfold SatisfiesAttributeConstraints, GetNRelSchema,
-  GetUnConstrRelation, DropQSConstraints in *.
-  generalize (rawAttrconstr (ith2 (rawRels r_o) idx)).
-  rewrite <- ith_imap2 in *.
-  destruct (attrConstraints (Vector.nth (qschemaSchemas qs_schema) idx)); eauto.
-Qed.
-
-Lemma refine_beq_RRecordType_dec :
-  forall rr : resourceRecord,
-    refine {b | decides b (rr!sTYPE = CNAME)}
-           (ret (beq_RRecordType rr!sTYPE CNAME)).
-Proof.
-  intros; rewrite <- beq_RRecordType_dec.
-  intros; refine pick val _.
-  finish honing.
-  find_if_inside; simpl; eauto.
-Qed.
-
-Lemma refine_constraint_check_into_query'' :
-  forall heading R P' P
-         (P_dec : DecideableEnsemble P),
-    Same_set _ (fun tup => P (indexedElement tup)) P'
-    -> refine
-         (Pick (fun (b : bool) =>
-                  decides b
-                          (exists tup2: @IndexedRawTuple heading,
-                              (R tup2 /\ P' tup2))))
-         (Bind
-            (Count (For (QueryResultComp R (fun tup => Where (P tup) Return tup))))
-            (fun count => ret (negb (beq_nat count 0)))).
-Proof.
-  Local Transparent Count.
-  unfold refine, Count, UnConstrQuery_In;
-    intros * excl * P_iff_P' pick_comp ** .
-  computes_to_inv; subst.
-
-  computes_to_constructor.
-
-  destruct (Datatypes.length v0) eqn:eq_length;
-    destruct v0 as [ | head tail ]; simpl in *; try discriminate; simpl.
-
-  pose proof (For_computes_to_nil _ R H).
-  rewrite not_exists_forall; intro a; rewrite not_and_implication; intros.
-  unfold not; intros; eapply H0; eauto; apply P_iff_P'; eauto.
-
-  apply For_computes_to_In with (x := head) in H; try solve [intuition].
-  destruct H as ( p & [ x0 ( in_ens & _eq ) ] ); subst.
-  eexists; split; eauto; apply P_iff_P'; eauto.
-
-  apply decidable_excl; assumption.
-Qed.
-
-Lemma refine_noDup_CNAME_check :
-  forall (rr : resourceRecord)
-         (R : @IndexedEnsemble resourceRecord),
-  (forall tup tup' : IndexedElement,
-          elementIndex tup <> elementIndex tup' ->
-          R tup ->
-          R tup' ->
-          (indexedElement tup)!sNAME = (indexedElement tup')!sNAME
-          -> (indexedElement tup)!sTYPE <> CNAME)
-  -> refine {b |
-            decides b
-                    (forall tup',
-                        R tup' ->
-                        rr!sNAME = (indexedElement tup')!sNAME -> rr!sTYPE <> CNAME)}
-           (If (beq_RRecordType rr!sTYPE CNAME)
-               Then count <- Count
-               For
-               (QueryResultComp R
-                                (fun tup => Where (rr!sNAME = tup!sNAME)
-                                                  Return tup )%QueryImpl);
-                  ret (beq_nat count 0) Else ret true).
-Proof.
-  intros.
-    intros; setoid_rewrite refine_pick_decides at 1;
-    [ | apply refine_is_CNAME__forall_to_exists | apply refine_not_CNAME__independent ].
-    setoid_rewrite refine_beq_RRecordType_dec; simplify with monad laws.
-    apply refine_If_Then_Else; eauto.
-    setoid_rewrite refine_constraint_check_into_query'' with (P := fun tup => rr!sNAME = tup!sNAME);
-    auto with typeclass_instances.
-    rewrite refineEquiv_bind_bind.
-    f_equiv.
-    unfold pointwise_relation; intros; simplify with monad laws;
-      rewrite <- negb_involutive_reverse; reflexivity.
-    intuition.
-  reflexivity.
-Qed.
-
-Corollary refine_noDup_CNAME_check_dns :
-  forall (rr : resourceRecord) r_o r_n,
-    @DropQSConstraints_AbsR DnsSchema r_o r_n
-  -> refine {b |
-            decides b
-                    (forall tup',
-                        (GetUnConstrRelation r_n Fin.F1) tup' ->
-                        rr!sNAME = (indexedElement tup')!sNAME -> rr!sTYPE <> CNAME)}
-           (If (beq_RRecordType rr!sTYPE CNAME)
-               Then count <- Count
-               For
-               (UnConstrQuery_In r_n Fin.F1
-                                (fun tup => Where (rr!sNAME = tup!sNAME)
-                                                  Return tup )%QueryImpl);
-                  ret (beq_nat count 0) Else ret true).
-Proof.
-  intros; eapply refine_noDup_CNAME_check.
-  intros; eapply (DropQSConstraints_AbsR_SatisfiesTupleConstraints _ _ H Fin.F1); eauto.
-Qed.
-
-Lemma is_empty_app {A} :
-  forall (l l' : list A),
-    is_empty (l ++ l') = andb (is_empty l) (is_empty l').
-Proof.
-  induction l; simpl; eauto.
-Qed.
-
-Lemma flatten_CompList_Prop {A}
-  : forall (P : Ensemble A) (P_dec : DecideableEnsemble P) (As As' : list A),
-    FlattenCompList.flatten_CompList (map (fun a : A => Where (P a)
-                                                              Return a ) As) ↝ As'
-    -> forall a, List.In a As' -> P a.
-Proof.
-  induction As; simpl; intros; computes_to_inv; subst; simpl in *; intuition.
-  unfold Query_Where, Query_Return in H; computes_to_inv; intuition.
-  destruct (dec a) eqn: ?.
-  - rewrite dec_decides_P in Heqb.
-    pose proof (H1 Heqb); computes_to_inv;
-      subst; simpl in *; subst; intuition eauto.
-    subst; eauto.
-  - apply Decides_false in Heqb; apply H2 in Heqb; subst; simpl in *;
-      eauto.
-Qed.
-
-Lemma flatten_CompList_Subset {A}
-  : forall (P : Ensemble A) (P_dec : DecideableEnsemble P) (As As' : list A),
-    FlattenCompList.flatten_CompList (map (fun a : A => Where (P a)
-                                                              Return a ) As) ↝ As'
-    -> forall a, List.In a As' -> List.In a As.
-Proof.
-  induction As; simpl; intros; computes_to_inv; subst; simpl in *; intuition.
-  unfold Query_Where, Query_Return in H; computes_to_inv; intuition.
-  destruct (dec a) eqn: ?.
-  - rewrite dec_decides_P in Heqb.
-    pose proof (H1 Heqb); computes_to_inv;
-      subst; simpl in *; subst; intuition eauto.
-  - apply Decides_false in Heqb; apply H2 in Heqb; subst; simpl in *;
-      eauto.
-Qed.
-
-Lemma flatten_CompList_nil {A}
-  : forall (P : Ensemble A) (P_dec : DecideableEnsemble P) (As : list A),
-    FlattenCompList.flatten_CompList
-      (map (fun a : A => Where (P a)
-                               Return a ) As) ↝ nil
-    -> forall a, List.In a As -> ~ P a.
-Proof.
-    induction As; simpl; intros; computes_to_inv; subst; simpl in *; intuition.
-    unfold Query_Where, Query_Return in H; computes_to_inv; intuition.
-    destruct (dec a) eqn: ?.
-    - rewrite dec_decides_P in Heqb.
-      apply H0 in Heqb; computes_to_inv;
-        subst; simpl in *; subst; intuition eauto.
-      discriminate.
-    - subst; apply H0 in H1; computes_to_inv;
-        subst; simpl in *; subst; intuition eauto.
-      discriminate.
-    - eapply IHAs; eauto.
-      apply app_eq_nil in H''; intuition; subst; eauto.
-Qed.
-
-Lemma refine_ListComprehension {A}
-  : forall (As : list A)
-           (P Q : A -> Prop),
-    (forall a, P a <-> Q a)
-    -> refine (⟦element in As | P element ⟧)
-              (⟦element in As | Q element ⟧).
-Proof.
-  induction As; simpl; intros; eauto.
-  - reflexivity.
-  - rewrite IHAs; eauto.
-    f_equiv; intro.
-    intros ? ?.
-    computes_to_inv; destruct v0; simpl in *.
-    + apply (@BindComputes _ _ _ _ true); eauto.
-      computes_to_econstructor; simpl; eauto.
-      apply H; assumption.
-    + apply (@BindComputes _ _ _ _ false); eauto.
-    computes_to_econstructor;
-      simpl; unfold UpperBound; intros.
-    intro; apply H0.
-    apply H; eassumption.
-Qed.
-
-Lemma refine_FindUpperBound {A B}
-  : forall (op : B -> B -> Prop)
-           (op_trans : forall b b' b'', op b b' -> op b' b'' -> op b b'')
-           (bound : B)
-           (As As' : list A)
-           (f : A -> B),
-    (forall a, List.In a As' -> op (f a) bound)
-    -> (exists a, List.In a As' /\ f a = bound)
-    -> refine (⟦element in As | UpperBound (fun a a' => op (f a) (f a')) As' element ⟧)
-              (⟦element in As | op bound (f element) ⟧).
-Proof.
-  intros.
-  unfold UpperBound.
-  apply refine_ListComprehension.
-  split; intros.
-  - destruct_ex; intuition eauto; subst; eauto.
-  - eapply op_trans; eauto.
-Qed.
-
-Lemma refine_MaxElements {A B}
-      {eqB : Query_eq B }
-  : forall (op : B -> B -> Prop)
-           (op_refl : forall b, op b b)
-           (op_trans : forall b b' b'', op b b' -> op b' b'' -> op b b'')
-           (op_dec : forall b, DecideableEnsemble (fun b' => op b' b))
-           (op_irrefl : forall b b', op b b' -> op b' b -> b = b')
-           (bound : B)
-           (As : @IndexedEnsemble A)
-           (f : A -> B),
-    refine (MaxElements (fun a a' => op (f a) (f a'))
-                        (As' <- {As' : list A | UnIndexedEnsembleListEquivalence As As'};
-                           FlattenCompList.flatten_CompList (map (fun a => Where (op (f a) bound)
-                                                                                 Return a) As')))
-           (As' <- (As' <- {As' : list A | UnIndexedEnsembleListEquivalence As As'};
-                      FlattenCompList.flatten_CompList (map (fun a => Where ((f a) = bound)
-                                                                            Return a) As'));
-              If negb (is_empty As') Then ret As' Else
-                 (MaxElements (fun a a' => op (f a) (f a'))
-                              (As' <- {As' : list A | UnIndexedEnsembleListEquivalence As As'};
-                                 FlattenCompList.flatten_CompList (map (fun a => Where (op (f a) bound /\ (f a) <> bound)
-                                                                                       Return a) As')))).
-Proof.
-  unfold MaxElements; intros; simplify with monad laws.
-  setoid_rewrite refineEquiv_bind_bind.
-  unfold refine; intros.
-  computes_to_inv.
-  destruct (is_empty v1) eqn: v1_eq; simpl in *; computes_to_inv; subst.
-  - computes_to_econstructor; eauto.
-    computes_to_econstructor; eauto.
-    assert (forall a', List.In a' v3 -> f a' <> bound).
-    { intros; eapply Permutation_in in H0;
-        eauto using (Permutation_UnIndexedEnsembleListEquivalence' H'' H).
-      clear H.
-      generalize dependent v1; generalize dependent v0; clear;
-        induction v0; simpl; intros; intuition;
-          computes_to_inv; subst.
-      + unfold Query_Where, Query_Return in H'; computes_to_inv; subst.
-        intuition; computes_to_inv; subst.
-        simpl in v1_eq; discriminate.
-      + eapply H0; eauto.
-        rewrite is_empty_app, andb_true_iff in v1_eq.
-        intuition.
-    }
-    generalize v2 H'''0 H0; clear; induction v3; simpl; intros;
-      computes_to_inv; subst; intuition eauto.
-    computes_to_econstructor.
-    eapply refine_Query_Where_Cond in H'''0; eauto.
-    intuition eauto.
-    computes_to_econstructor.
-    eapply IHv3; eauto.
-    eauto.
-  - computes_to_econstructor; eauto.
-    assert (exists v',
-               computes_to
-                 (FlattenCompList.flatten_CompList (map (fun a : A => Where (op (f a) bound)
-                                                                         Return a ) v0)) v').
-    {
-      revert op_dec; clear; induction v0; simpl; intros; eauto.
-      destruct IHv0; eauto.
-      destruct (dec (DecideableEnsemble := op_dec bound) (f a)) eqn:?.
-      rewrite dec_decides_P in Heqb.
-      eexists; computes_to_econstructor.
-      computes_to_econstructor; split; intros.
-      computes_to_econstructor.
-      intuition.
-      computes_to_econstructor; eauto.
-      eexists; computes_to_econstructor.
-      computes_to_econstructor; split; intros.
-      apply Decides_false in Heqb.
-      intuition.
-      reflexivity.
-      computes_to_econstructor; eauto.
-    }
-    destruct_ex; computes_to_econstructor; eauto.
-    eapply (refine_FindUpperBound _ op_trans bound); eauto.
-    intros.
-    eapply flatten_CompList_Prop in H0; eauto.
-    refine {| dec a := dec (f a) |}.
-    intros; rewrite dec_decides_P; reflexivity.
-    generalize dependent v; generalize dependent x; clear H.
-    induction v0; simpl.
-    + intros; computes_to_inv; subst; simpl in *; discriminate.
-    + intros; computes_to_inv; subst; simpl; eauto.
-      unfold Query_Where, Query_Return in H0, H'; computes_to_inv; subst.
-      intuition; computes_to_inv; subst.
-      destruct (A_eq_dec (f a) bound); subst.
-      * specialize (H0 (eq_refl _)); computes_to_inv; subst.
-        specialize (H (op_refl _)); computes_to_inv; subst.
-        eexists; simpl; intuition eauto.
-      * apply H2 in n; subst.
-        simpl in v1_eq.
-        destruct (IHv0 _ H0' _ H'' v1_eq); intuition.
-        eexists; split; eauto.
-        apply in_or_app; right; eauto.
-    + generalize dependent v; generalize dependent x; clear H.
-      induction v0; simpl.
-      * intros; computes_to_inv; subst; simpl in *; discriminate.
-      * intros; computes_to_inv; subst; simpl; eauto.
-        unfold Query_Where, Query_Return in H0, H'; computes_to_inv; subst.
-        intuition; computes_to_inv; subst.
-        destruct (dec (DecideableEnsemble := op_dec bound) (f a)) eqn:?.
-        rewrite dec_decides_P in Heqb; pose proof (H Heqb).
-        computes_to_inv; subst; simpl.
-        destruct (A_eq_dec (f a) bound); subst.
-        pose proof (H0 (eq_refl _)); computes_to_inv; subst.
-        destruct (is_empty v2) eqn: ?.
-        apply (@BindComputes _ _ _ _ [ ]); eauto.
-        { revert eqB op_dec op_irrefl Heqb0 H0' H''; clear; revert v4 v2; induction v0;
-            simpl; intros; computes_to_inv; subst; simpl.
-          computes_to_econstructor.
-          unfold Query_Where, Query_Return in H0', H''; computes_to_inv; subst.
-          intuition; computes_to_inv; subst.
-          destruct (dec (DecideableEnsemble := op_dec (f a)) (f a0)) eqn: ?.
-          - rewrite dec_decides_P in Heqb; pose proof (H Heqb).
-            computes_to_inv; subst.
-            simpl.
-            destruct (A_eq_dec (f a0) (f a)).
-            + apply H1 in e; computes_to_inv; subst.
-              simpl in *; discriminate.
-            + pose proof (H2 n); subst; simpl in *.
-              computes_to_econstructor; eauto.
-              apply (@BindComputes _ _ _ _ false); eauto.
-              computes_to_econstructor; simpl.
-              intuition.
-          - apply Decides_false in Heqb.
-            pose proof (H0 Heqb); subst; simpl.
-            destruct (A_eq_dec (f a0) (f a)); subst.
-            intuition; computes_to_inv; subst.
-            simpl in Heqb0; discriminate.
-            apply H2 in n; subst; eauto.
-        }
-        apply (@BindComputes _ _ _ _ true); eauto.
-        destruct v2; simpl in *; try discriminate.
-        computes_to_econstructor.
-        computes_to_econstructor.
-        eauto.
-        apply (@BindComputes _ _ _ _ true); eauto.
-        pose proof (H2 n); subst; simpl.
-        simpl in v1_eq.
-        computes_to_econstructor; eauto.
-        apply (@BindComputes _ _ _ _ false); eauto.
-        computes_to_econstructor; simpl.
-        intro; eapply n; eauto.
-        apply Decides_false in Heqb.
-        pose proof (H1 Heqb); subst; simpl.
-        destruct (A_eq_dec (f a) bound); subst.
-        intuition.
-        apply H2 in n; subst; eauto.
-Qed.
-
-Lemma Query_Where_And_Sym {ResultT}
-  : forall (P Q : Prop)
-           (body : Comp (list ResultT)),
-    refine (Query_Where (P /\ Q) body)
-           (Query_Where (Q /\ P) body).
-Proof.
-  intros; rewrite refine_Query_Where_Cond;
-    try reflexivity; intuition.
-Qed.
 
 Ltac implement_insert'' :=
   implement_insert' ltac:(CombineCase5 StringPrefixIndexUse EqIndexUse)
@@ -541,23 +144,84 @@ Proof.
     eapply refineFueledFix.
     - finish honing.
     - intros.
+      etransitivity.
+      etransitivity.
+      rewrite (@MaxElementsUnConstrQuery_In DnsSchema Fin.F1 (fun r : resourceRecord => GetAttributeRaw r Fin.F1) a1 r_o).
       doOne ltac:(drop_constraints)
                    drop_constraints_drill ltac:(repeat subst_refine_evar; cbv beta; simpl; try finish honing).
-      doAny ltac:(drop_constraints)
+      drop_constraints_drill.
+      drop_constraints_from_query'.
+      finish honing.
+      setoid_rewrite refine_If_Then_Else_Bind; simpl.
+      match goal with
+        |- refine (If_Then_Else ?c _ _) _ =>
+        subst_refine_evar; eapply refine_if with (b := c);
+          let H := fresh in
+          intro H; set_refine_evar; try rewrite H; simpl
+      end.
+      { simplify with monad laws.
+        rewrite refine_If_Then_Else_false.
+        etransitivity.
+        apply refine_IfDec_true.
+        apply (For_In_Where_Prop _ H3).
+        finish honing.
+        rewrite <- negb_false_iff, <- negb_involutive_reverse in H4.
+        apply H4.
+      }
+      { eapply refine_under_bind_both_ambivalent with
+        (c' := MaxElements (fun r r' : @RawTuple {| NumAttr := 4; AttrList := [DomainName : Type ; timeT : Type; RRecordClass : Type; RDataType : Type]%NamedSchema |} => prefix (GetAttributeRaw r Fin.F1) (GetAttributeRaw r' Fin.F1))
+              For (Query_In r_o Fin.F1
+                     (fun r : RawTuple =>
+                        Where (
+                            RDataTypeToRRecordType (GetAttributeRaw r (Fin.FS (Fin.FS (Fin.FS Fin.F1)))) = NS
+                            /\ prefix (GetAttributeRaw r Fin.F1) a1
+                            /\ GetAttributeRaw r Fin.F1 <> a1)
+                      Return r ))).
+        intros.
+        eexists a'; split.
+        clear; admit.
+        match goal with
+          |- refine (If_Then_Else ?c _ _) _ =>
+          subst_refine_evar; eapply refine_if with (b := c);
+            let H := fresh in
+            intro H; set_refine_evar; try rewrite H; simpl
+        end.
+        finish honing.
+        setoid_rewrite H2.
+        rewrite refine_IfDec with (b := false); simpl.
+        drop_constraints_drill.
+        finish honing.
+        doOne ltac:(drop_constraints)
+                     drop_constraints_drill ltac:(repeat subst_refine_evar; cbv beta; simpl; try finish honing).
+        doOne ltac:(drop_constraints)
+                     drop_constraints_drill ltac:(repeat subst_refine_evar; cbv beta; simpl; try finish honing).
+      doOne ltac:(drop_constraints)
                    drop_constraints_drill ltac:(repeat subst_refine_evar; cbv beta; simpl; try finish honing).
+      doOne ltac:(drop_constraints)
+                   drop_constraints_drill ltac:(repeat subst_refine_evar; cbv beta; simpl; try finish honing).
+      rewrite Forall_forall.
+      intro.
+      unfold MaxElements in H6; computes_to_inv.
+      pose proof (For_In_Where_Prop (qs_schema := DnsSchema) _ H6).
+      rewrite Forall_forall in H10.
+      clear; admit.
+      }
+      simpl.
+      drop_constraints_drill.
+      finish honing.
+      drop_constraints_drill.
+      finish honing.
+      doOne ltac:(drop_constraints)
+                   drop_constraints_drill ltac:(repeat subst_refine_evar; cbv beta; simpl; try finish honing).
+      doOne ltac:(drop_constraints)
+                   drop_constraints_drill ltac:(repeat subst_refine_evar; cbv beta; simpl; try finish honing).
+      doOne ltac:(drop_constraints)
+                   drop_constraints_drill ltac:(repeat subst_refine_evar; cbv beta; simpl; try finish honing).
+      finish honing.
+      finish honing.
+      finish honing.
       setoid_rewrite H2.
-      doOne ltac:(drop_constraints)
-                   drop_constraints_drill ltac:(repeat subst_refine_evar; cbv beta; simpl; try finish honing).
-      doOne ltac:(drop_constraints)
-                   drop_constraints_drill ltac:(repeat subst_refine_evar; cbv beta; simpl; try finish honing).
-      doOne ltac:(drop_constraints)
-                   drop_constraints_drill ltac:(repeat subst_refine_evar; cbv beta; simpl; try finish honing).
-      doOne ltac:(drop_constraints)
-                   drop_constraints_drill ltac:(repeat subst_refine_evar; cbv beta; simpl; try finish honing).
-      doOne ltac:(drop_constraints)
-                   drop_constraints_drill ltac:(repeat subst_refine_evar; cbv beta; simpl; try finish honing).
-      doAny ltac:(drop_constraints)
-                   drop_constraints_drill ltac:(repeat subst_refine_evar; cbv beta; simpl; try finish honing).
+      simpl; finish honing.
     - Local Opaque encode_packet_Spec.
       doAny ltac:(drop_constraints)
                    drop_constraints_drill ltac:(repeat subst_refine_evar; cbv beta; simpl; try finish honing).
@@ -570,9 +234,16 @@ Proof.
       doOne ltac:(drop_constraints)
                    drop_constraints_drill ltac:(repeat subst_refine_evar; cbv beta; simpl; try finish honing).
   }
+  Local Opaque SumType.SumType_index.
+  Local Opaque SumType.SumType_proj.
+  Local Opaque SumType.inj_SumType.
 
-  hone representation using (@DecomposeRawQueryStructureSchema_AbsR _ DnsSchema Fin.F1 (Fin.FS (Fin.FS (Fin.FS (Fin.F1)))) id
-             id).
+  hone representation using (@DecomposeRawQueryStructureSchema_AbsR
+                               _ DnsSchema Fin.F1 (Fin.FS (Fin.FS (Fin.FS (Fin.F1)))) _
+                               (SumType.SumType_index ResourceRecordTypeTypes)
+                               (SumType.SumType_proj ResourceRecordTypeTypes)
+                               (SumType.inj_SumType ResourceRecordTypeTypes)
+                            ).
   { simplify with monad laws.
     refine pick val _.
     2: apply DecomposeRawQueryStructureSchema_empty_AbsR.
@@ -581,8 +252,8 @@ Proof.
   {
     simplify with monad laws.
     drop_constraints_drill.
-    rewrite (refine_UnConstrFreshIdx_DecomposeRawQueryStructureSchema_AbsR_Equiv H0);
-      finish honing.
+    rewrite (refine_UnConstrFreshIdx_DecomposeRawQueryStructureSchema_AbsR_Equiv H0 Fin.F1).
+    finish honing.
     drop_constraints_drill.
     drop_constraints_drill.
     setoid_rewrite refine_Iterate_Equiv_QueryResultComp; try eassumption.
@@ -591,9 +262,9 @@ Proof.
     finish honing.
     drop_constraints_drill.
     setoid_rewrite Query_Where_And_Sym.
-    setoid_rewrite (refine_QueryIn_Where H0).
+    setoid_rewrite (refine_QueryIn_Where _ _ H0).
     simpl.
-    unfold Tuple_DecomposeRawQueryStructure_inj; simpl.
+    unfold Tuple_DecomposeRawQueryStructure_inj'; simpl.
     unfold GetAttribute, GetAttributeRaw at 2; simpl.
     unfold ilist2_hd; simpl.
     finish honing.
@@ -615,17 +286,47 @@ Proof.
   { simplify with monad laws.
     drop_constraints_drill.
     finish honing.
+    rewrite !refine_If_Opt_Then_Else_Bind.
     drop_constraints_drill.
-    drop_constraints_drill.
+    simplify with monad laws.
     drop_constraints_drill.
     eapply refineFueledFix.
     finish honing.
     intros.
+    rewrite (refine_Iterate_Equiv_QueryResultComp _ H0).
+    drop_constraints_drill.
+    finish honing.
+    drop_constraints_drill.
+    setoid_rewrite H2.
+    finish honing.
     simplify with monad laws.
-    (Fin.FS (Fin.FS (Fin.FS (Fin.FS (Fin.F1)))))
-  ).
-  Print DnsSchema.
-  hone representation using (@DecomposeRawQueryStructureSchema_AbsR _ DnsSchema (Fin.FS (Fin.FS (Fin.FS Fin.F1))))
+    setoid_rewrite (refine_QueryIn_Where _ _ H0).
+    drop_constraints_drill.
+    simpl.
+    unfold Tuple_DecomposeRawQueryStructure_inj'; simpl.
+    unfold GetAttribute, GetAttributeRaw; simpl.
+    unfold ilist2_hd; simpl.
+    finish honing.
+    drop_constraints_drill.
+    finish honing.
+    drop_constraints_drill.
+    finish honing.
+    drop_constraints_drill.
+    finish honing.
+    rewrite (refine_Iterate_Equiv_QueryResultComp _ H0).
+    finish honing.
+    drop_constraints_drill.
+    finish honing.
+    simpl; refine pick val _; try eassumption.
+    simplify with monad laws.
+    finish honing.
+    simplify with monad laws.
+    simpl; refine pick val _; try eassumption.
+    simplify with monad laws.
+    finish honing.
+  }
+  simpl.
+
 
 
   make_simple_indexes ({|prim_fst := [(FindStringPrefixIndex, @Fin.F1 4)];
