src/Examples/DnsServer/MinimalDNSServer.v
@@ -146,3 +146,4 @@ Proof.
 
 Time Definition DNSImpl := Eval simpl in (projT1 DnsManual).
 Print DNSImpl.
+v
